irreducible tags

SP1Chips/Addw/Constraints.lean
@@ -7,7 +7,7 @@ namespace Addw
 section constraints
 
 -- Generated Lean code for chip AddwChip
-def constraints (Main : Vector (Fin BB) 37) : SP1ConstraintList :=
+@[irreducible] def constraints (Main : Vector (Fin BB) 37) : SP1ConstraintList :=
   let E0 : Fin BB := Main[36] - 1
   let E1 : Fin BB := Main[36] * E0
   let E2 : Fin BB := 4 * Main[31]
