SP1Chips/Bitwise/Constraints.lean
@@ -12,7 +12,7 @@ def is_real : Prop := Main[48] = 1 ∨ Main[49] = 1 ∨ Main[50] = 1
 section constraints
 
 -- Generated Lean code for chip BitwiseChip
-def constraints (Main : Vector (Fin BB) 52) : SP1ConstraintList :=
+@[irreducible] def constraints (Main : Vector (Fin BB) 52) : SP1ConstraintList :=
   let E0 : Fin BB := Main[49] + Main[50]
   let E1 : Fin BB := E0 + Main[51]
   let E2 : Fin BB := Main[49] - 1
@@ -71,6 +71,22 @@ def constraints (Main : Vector (Fin BB) 52) : SP1ConstraintList :=
   ]
 
 end constraints
+
+lemma allHold_constraints_iff :
+  List.Forall SP1Constraint.toProp (constraints Main) ↔
+    let ret_val := (BitwiseU16Operation.constraints #v[Main[15], Main[16], Main[17], Main[18]] #v[Main[25], Main[26], Main[27], Main[28]] { b_low_bytes := { low_bytes := #v[Main[32], Main[33], Main[34], Main[35]] }, c_low_bytes := { low_bytes := #v[Main[36], Main[37], Main[38], Main[39]] }, bitwise_operation := { result := #v[Main[40], Main[41], Main[42], Main[43], Main[44], Main[45], Main[46], Main[47]] } } (Main[48] * 2 + Main[49] * 1 + Main[50] * 0) (Main[48] + Main[49] + Main[50])).1
+    List.Forall SP1Constraint.toProp (BitwiseU16Operation.constraints #v[Main[15], Main[16], Main[17], Main[18]] #v[Main[25], Main[26], Main[27], Main[28]] { b_low_bytes := { low_bytes := #v[Main[32], Main[33], Main[34], Main[35]] }, c_low_bytes := { low_bytes := #v[Main[36], Main[37], Main[38], Main[39]] }, bitwise_operation := { result := #v[Main[40], Main[41], Main[42], Main[43], Main[44], Main[45], Main[46], Main[47]] } } (Main[48] * 2 + Main[49] * 1 + Main[50] * 0) (Main[48] + Main[49] + Main[50])).2 ∧
+    List.Forall SP1Constraint.toProp (CPUState.constraints { clk_high := Main[0], clk_16_24 := Main[1], clk_0_16 := Main[2], pc := #v[Main[3], Main[4], Main[5]] } #v[(Main[3] + 4), Main[4], Main[5]] 8 (Main[48] + Main[49] + Main[50])) ∧
+    List.Forall SP1Constraint.toProp (ALUTypeReader.constraints Main[0] (Main[2] + Main[1] * 65536) #v[Main[3], Main[4], Main[5]] (Main[48] * 3 + Main[49] * 4 + Main[50] * 5) #v[Main[51], (Main[48] * 4 + Main[49] * 6 + Main[50] * 7), 0, 0] #v[ret_val[0], ret_val[1], ret_val[2], ret_val[3]] { op_a := Main[6], op_a_memory := { prev_value := #v[Main[7], Main[8], Main[9], Main[10]], access_timestamp := { prev_low := Main[11], diff_low_limb := Main[12] } }, op_a_0 := Main[13], op_b := Main[14], op_b_memory := { prev_value := #v[Main[15], Main[16], Main[17], Main[18]], access_timestamp := { prev_low := Main[19], diff_low_limb := Main[20] } }, op_c := #v[Main[21], Main[22], Main[23], Main[24]], op_c_memory := { prev_value := #v[Main[25], Main[26], Main[27], Main[28]], access_timestamp := { prev_low := Main[29], diff_low_limb := Main[30] } }, imm_c := Main[31], is_trusted := sorry } (Main[48] + Main[49] + Main[50])) ∧
+    (Main[48] = 0 ∨ Main[48] = 1) ∧
+    (Main[49] = 0 ∨ Main[49] = 1) ∧
+    (Main[50] = 0 ∨ Main[50] = 1) ∧
+    (Main[48] + Main[49] + Main[50] = 0 ∨ Main[48] + Main[49] + Main[50] - 1 = 0) ∧
+    (Main[48] + Main[49] + Main[50] = 0 ∨ Main[51] - (Main[31] * (Main[48] * 19 + Main[49] * 19 + Main[50] * 19) + (1 - Main[31]) * (Main[48] * 51 + Main[49] * 51 + Main[50] * 51)) = 0)
+  := by
+    stop
+    simp [constraints]
+    split; constructor <;> simp_all [sub_eq_zero]
 
 section opcodes
 
