SP1Chips/Load/LoadHalf/Constraints.lean
@@ -11,7 +11,7 @@ namespace LoadHalf
 section constraints
 
 -- Generated Lean code for chip LoadHalfChip
-def constraints (Main : Vector (Fin BB) 46) : SP1ConstraintList :=
+@[irreducible] def constraints (Main : Vector (Fin BB) 46) : SP1ConstraintList :=
   let E0 : Fin BB := Main[1] * 65536
   let E1 : Fin BB := Main[2] + E0
   let E2 : Fin BB := 20 * Main[43]
