SP1Chips/ShiftLeft/Constraints.lean
@@ -12,7 +12,7 @@ def is_real : Prop := Main[62] = 1 ∨ Main[63] = 1
 section constraints
 
 -- Generated Lean code for chip ShiftLeftChip
-def constraints (Main : Vector (Fin BB) 66) : SP1ConstraintList :=
+@[irreducible] def constraints (Main : Vector (Fin BB) 66) : SP1ConstraintList :=
   let E0 : Fin BB := Main[63] + Main[64]
   let E1 : Fin BB := E0 - 1
   let E2 : Fin BB := E0 * E1
@@ -287,7 +287,7 @@ lemma cancel_mul_65536 { a b c x : Fin BB } (h_dvd : (x : ℕ) ∣ 65536) : a * 
   := by
   obtain ⟨ z, h_eq ⟩ := h_dvd; rw [h_eq]
   have x_pos : 0 < (x : ℕ) := by nlinarith
-  have xz_BB : (x : ℕ) * z < 2013265921 := by nlinarith
+  have xz_BB : (x : ℕ) * z < 2130706433 := by nlinarith
   have h_eq_BB : 65536 = x * z := by simp [Fin.ext_iff, Fin.mul_def]; omega
   rw [h_eq_BB]
   rw [mul_comm x z, ← mul_assoc, ← right_distrib]
@@ -305,7 +305,7 @@ lemma is_mod_64 {c0 m : Fin BB} : m < 64 → c0 < 65536 → ((c0 - m) * 19818086
   . simp [BitVec.toNat_eq] at this
     repeat rw [Nat.mod_eq_of_lt (b := 18446744073709551616) (by omega)] at this
     assumption
-  . suffices : ((2013265921 - BitVec.ofNat 64 ↑m) * BitVec.ofNat 64 1981808641 + BitVec.ofNat 64 ↑c0 * 1981808641#64) % 2013265921#64 < 1024#64
+  . suffices : ((2130706433 - BitVec.ofNat 64 ↑m) * BitVec.ofNat 64 1981808641 + BitVec.ofNat 64 ↑c0 * 1981808641#64) % 2130706433#64 < 1024#64
     . clear hdiff
       have : BitVec.ofNat 64 c0.val < 65536 := by simp; omega
       have : BitVec.ofNat 64 m.val < 64 := by simp; omega
@@ -547,10 +547,10 @@ lemma spec.sll (h : is_sll Main) :
       rw [Word.toBitVec64_toNat]
       . simp [Word.toNat]
         try simp [Fin.val_add, Fin.val_mul] at b0_16 b1_16 b2_16 b3_16 ⊢
-        repeat rw [Nat.mod_eq_of_lt (b := 2013265921) (by omega)]
+        repeat rw [Nat.mod_eq_of_lt (b := 2130706433) (by omega)]
         omega
       . apply Word.isU64_of_cases <;> simp [Fin.val_add, Fin.val_mul] <;>
-        (repeat rw [Nat.mod_eq_of_lt (b := 2013265921) (by omega)]) <;>
+        (repeat rw [Nat.mod_eq_of_lt (b := 2130706433) (by omega)]) <;>
         omega
     }
 
@@ -662,10 +662,10 @@ lemma spec.slli (h : is_slli Main) :
       rw [Word.toBitVec64_toNat]
       . simp [Word.toNat]
         try simp [Fin.val_add, Fin.val_mul] at b0_16 b1_16 b2_16 b3_16 ⊢
-        repeat rw [Nat.mod_eq_of_lt (b := 2013265921) (by omega)]
+        repeat rw [Nat.mod_eq_of_lt (b := 2130706433) (by omega)]
         omega
       . apply Word.isU64_of_cases <;> simp [Fin.val_add, Fin.val_mul] <;>
-        (repeat rw [Nat.mod_eq_of_lt (b := 2013265921) (by omega)]) <;>
+        (repeat rw [Nat.mod_eq_of_lt (b := 2130706433) (by omega)]) <;>
         omega
     }
 
@@ -775,7 +775,7 @@ lemma spec.sllw (h : is_sllw Main) :
       rcases b_cb0 <;> rcases b_cb1 <;> rcases b_cb2 <;>
       rcases b_cb3 <;> rcases b_cb4 <;> simp_all <;>
       apply HWord.isU32_of_cases <;> simp_all [Fin.val_add, Fin.val_mul] <;>
-      (repeat rw [Nat.mod_eq_of_lt (b := 2013265921) (by omega)]) <;>
+      (repeat rw [Nat.mod_eq_of_lt (b := 2130706433) (by omega)]) <;>
       omega
 
     have ⟨ _, _ ⟩ := HWord.lt_cases_of_isU32 h_isU32_a
@@ -807,7 +807,7 @@ lemma spec.sllw (h : is_sllw Main) :
           (try apply cancel_mul_65536 (by simp) at h_b3_dec)
           simp_all [HWord.toNat]
           try simp [Fin.val_add, Fin.val_mul] at b0_16 b1_16 b2_16 b3_16 ⊢
-          repeat rw [Nat.mod_eq_of_lt (b := 2013265921) (by omega)]
+          repeat rw [Nat.mod_eq_of_lt (b := 2130706433) (by omega)]
           omega
         }
 
@@ -917,7 +917,7 @@ lemma spec.slliw (h : is_slliw Main) :
       rcases b_cb0 <;> rcases b_cb1 <;> rcases b_cb2 <;>
       rcases b_cb3 <;> rcases b_cb4 <;> simp_all <;>
       apply HWord.isU32_of_cases <;> simp_all [Fin.val_add, Fin.val_mul] <;>
-      (repeat rw [Nat.mod_eq_of_lt (b := 2013265921) (by omega)]) <;>
+      (repeat rw [Nat.mod_eq_of_lt (b := 2130706433) (by omega)]) <;>
       omega
 
     have ⟨ _, _ ⟩ := HWord.lt_cases_of_isU32 h_isU32_a
@@ -949,7 +949,7 @@ lemma spec.slliw (h : is_slliw Main) :
           (try apply cancel_mul_65536 (by simp) at h_b3_dec)
           simp_all [HWord.toNat]
           try simp [Fin.val_add, Fin.val_mul] at b0_16 b1_16 b2_16 b3_16 ⊢
-          repeat rw [Nat.mod_eq_of_lt (b := 2013265921) (by omega)]
+          repeat rw [Nat.mod_eq_of_lt (b := 2130706433) (by omega)]
           omega
         }
 
