SP1Operations/Operation/BitwiseU16Operation.lean
@@ -36,7 +36,7 @@ lemma spec.and
       rw [Word.and_toBWord h_isU64_b h_isU64_cc]
       simp [Word.toBitVec64, Word.toNat, Word.toBWord, BWord.toBitVec64, BWord.toNat]
       simp [Fin.val_add, Fin.val_mul]
-      repeat rw [Nat.mod_eq_of_lt (b := 2013265921) (by omega)]
+      repeat rw [Nat.mod_eq_of_lt (b := 2130706433) (by omega)]
       rw [Fin.lt_iff_val_lt_val, Fin.mod_val] at hb0 hc0 hb2 hc2 hb4 hc4 hb6 hc6
       rw [Fin.lt_iff_val_lt_val, Fin.div_val] at hb1 hc1 hb3 hc3 hb5 hc5 hb7 hc7
       simp_all
@@ -77,7 +77,7 @@ lemma spec.or
       rw [Word.or_toBWord h_isU64_b h_isU64_cc]
       simp [Word.toBitVec64, Word.toNat, Word.toBWord, BWord.toBitVec64, BWord.toNat]
       simp [Fin.val_add, Fin.val_mul]
-      repeat rw [Nat.mod_eq_of_lt (b := 2013265921) (by omega)]
+      repeat rw [Nat.mod_eq_of_lt (b := 2130706433) (by omega)]
       rw [Fin.lt_iff_val_lt_val, Fin.mod_val] at hb0 hc0 hb2 hc2 hb4 hc4 hb6 hc6
       rw [Fin.lt_iff_val_lt_val, Fin.div_val] at hb1 hc1 hb3 hc3 hb5 hc5 hb7 hc7
       simp_all
@@ -118,7 +118,7 @@ lemma spec.xor
       rw [Word.xor_toBWord h_isU64_b h_isU64_cc]
       simp [Word.toBitVec64, Word.toNat, Word.toBWord, BWord.toBitVec64, BWord.toNat]
       simp [Fin.val_add, Fin.val_mul]
-      repeat rw [Nat.mod_eq_of_lt (b := 2013265921) (by omega)]
+      repeat rw [Nat.mod_eq_of_lt (b := 2130706433) (by omega)]
       rw [Fin.lt_iff_val_lt_val, Fin.mod_val] at hb0 hc0 hb2 hc2 hb4 hc4 hb6 hc6
       rw [Fin.lt_iff_val_lt_val, Fin.div_val] at hb1 hc1 hb3 hc3 hb5 hc5 hb7 hc7
       simp_all
